Prove some Real lemmas, make assumptions clearer for others

src/lib/kuiper/Kuiper.Real.fsti
@@ -10,13 +10,19 @@ does not expose one. *)
 val rexp (x:real) : real
 val rlog (x:real{x >. 0.0R}) : real
 
-val rexp_pos (x:real)
-: Lemma (ensures rexp x >. 0.0R)
-        [SMTPat (rexp x)]
+(* Usual math laws about exponentiation and logarithms. *)
 
-(* Usual math laws about exponentiation and logarithms.  We don't prove these
-because we can't--- F* reals are very opaque. Though we could reduce the
-number of axioms a bit, and upstream it. *)
+val rexp_positive (x : real)
+  : Lemma (ensures rexp x >. 0.0R)
+          [SMTPat (rexp x)]
+
+val rexp_base ()
+  : Lemma (rexp 0.0R == 1.0R)
+
+val exp_add (x y : real)
+  : Lemma (ensures rexp (x +. y) == rexp x *. rexp y)
+          [SMTPat (rexp (x +. y))]
+
 val log_exp (x : real)
   : Lemma (ensures rlog (rexp x) == x)
           [SMTPat (rlog (rexp x))]
@@ -24,10 +30,6 @@ val log_exp (x : real)
 val exp_log (x : real{x >. 0.0R})
   : Lemma (ensures rexp (rlog x) == x)
           [SMTPat (rexp (rlog x))]
-
-val exp_add (x y : real)
-  : Lemma (ensures rexp (x +. y) == rexp x *. rexp y)
-          [SMTPat (rexp (x +. y))]
 
 val exp_sub (x y : real)
   : Lemma (ensures rexp (x -. y) == rexp x /. rexp y)
@@ -43,14 +45,9 @@ val log_div (x y : real{x >. 0.0R /\ y >. 0.0R})
 
 let rsum (s : Seq.seq real) : real = seq_fold_left (+.) 0.0R s
 
-let rec sum_non_zero
+val sum_non_zero
     (s : Seq.seq real { forall (i:natlt (Seq.length s)). Seq.index s i >. 0.0R })
-    (acc:real)
+    (acc : real)
   : Lemma (requires Seq.length s > 0)
           (ensures seq_fold_left (+.) acc s >. acc)
-          (decreases Seq.length s)
           [SMTPat (seq_fold_left (+.) acc s)]
-  = if Seq.length s = 1 then ()
-    else
-      let SCons hd tl = view_seq s in
-      sum_non_zero tl (acc +. hd <: real)
